made more proofs work

lib/stack.ml
@@ -1,23 +1,20 @@
 
 type 'a t = {
   mutable contents: 'a list;
-  mutable length: int
 }
 
 let create () = {
   contents=[];
-  length=0
 }
 
 let push st x =
-  st.contents <- x :: st.contents;
-  st.length <- st.length + 1
+  st.contents <- x :: st.contents
   
 let pop st =
   match st.contents with
   | [] -> None
   | h :: t ->
     st.contents <- t;
-    st.length <- st.length - 1;
     Some h
-      
+
+let length st = List.length st
