src/main.ml
@@ -1,4 +1,6 @@
 
+open Core
 
-let ()  =
+let ()  = 
+
   Printf.printf "hello world!"
